TangleLearning_Search.thy
@@ -42,6 +42,32 @@ lemmas search_step_induct[consumes 1, case_names step] =
     where P="\<lambda>(a,b) (c,d). P a b c d" for P,
     unfolded split]
 
+(** The search algorithm applies the search_step until it reaches the end.
+    We do not have to specify that ({},Y) is not in the domain of the step,
+    as this follows automatically because no further steps exist from an empty R. *)
+definition search :: "'v set \<Rightarrow> 'v set set \<Rightarrow> bool" where
+  "search R Y \<equiv> search_step\<^sup>*\<^sup>* (R,{}) ({},Y)"
+
+
+section \<open>Invariant\<close>
+(** TODO: invariant, prove property of Y on termination. *)
+(** The current invariant states that everything contained in Y is a tangle.
+    This should probably be restated to say that everything contained in Y is a tangle with its
+    corresponding strategy. *)
+(**
+definition search_I ::  "'v set \<times> 'v set set \<Rightarrow> bool" where
+  "search_I S \<equiv> finite (snd S) \<and> (\<forall>U \<in> snd S. \<exists>\<alpha>. tangle \<alpha> U) \<and> (fst S={} \<longrightarrow> \<dots>)"
+*)
+
+definition search_I :: "'v set \<times> 'v set set \<Rightarrow> bool" where
+  "search_I \<equiv> \<lambda>(R,Y). finite R \<and> valid_subgame R \<and> finite Y \<and> (\<forall>U \<in> Y. \<exists>\<alpha>. tangle \<alpha> U \<and> U \<notin> T)"
+
+(** If we end with an empty region, then we have a finite, non-empty Y containing new tangles that
+    were not included in T before, as specified by our invariant. *)
+lemma search_I_correct:
+  "search_I ({},Y) \<Longrightarrow> finite Y \<and> Y \<noteq> {} \<and> (\<forall>U \<in> Y. \<exists>\<alpha>. tangle \<alpha> U \<and> U \<notin> T)"
+  unfolding search_I_def apply simp sorry
+
 (** If the initial R is finite, then R' is finite after a step. *)
 lemma search_step_R_finite:
   "\<lbrakk>search_step (R,Y) (R',Y'); finite R\<rbrakk> \<Longrightarrow> finite R'"
@@ -64,151 +90,6 @@ proof (induction rule: search_step_induct)
 
   ultimately show ?case ..
 qed
-
-(*
-(** search_step is inversely monotonous on R: R strictly decreases with every step. *)
-lemma search_step_R_anti_mono: "search_step S S' \<Longrightarrow> fst S' \<subset> fst S"
-proof (induction rule: search_step.induct)
-  case (step R p \<alpha> A T\<^sub>\<alpha> Z \<sigma> V\<^sub>\<alpha> V\<^sub>\<beta> Ov Y' Y R')
-  (** We know that every t in T\<^sub>\<alpha> is a tangle in the subgame of R, and that T\<^sub>\<alpha> is finite. We need
-      these properties for showing the next two properties. *)
-  from step(7) have tangles_T\<^sub>\<alpha>: "\<forall>t\<in>T\<^sub>\<alpha>. paritygame.tangle (Restr E R) (V \<inter> R) (V\<^sub>0 \<inter> R) pr \<alpha> t"
-    by blast
-  from step(7) have fin_T\<^sub>\<alpha>: "finite T\<^sub>\<alpha>"
-    using finite_subset[OF _ fin_T] by simp
-  (** We show that Z is not empty. *)
-  have "Z \<noteq> {}" proof -
-    (** R is finite *)
-    from finite_subset[OF step(2) fin_V] have fin_R: "finite R" .
-    (** A is part of the finite non-empty set R, therefore, it must contain at least one node
-        with priority p, and thus it is not empty. *)
-    from step(6) step(4) have "A \<noteq> {}"
-      using pr_set_exists[OF fin_R step(1)] by blast
-    (** Since the target A is part of the tangle-attracted region Z, Z must also be non-empty. *)
-    with paritygame.target_in_tangle_attractor[OF step(3) tangles_T\<^sub>\<alpha> fin_T\<^sub>\<alpha> step(8)]
-    show ?thesis by auto
-  qed
-  (** Furthermore, Z is a subset of of R. *)
-  moreover have "Z \<subseteq> R" proof -
-    from step(6) have A_in_R: "A \<subseteq> R" by simp
-    (** Since the tangle-attracted Z region is a subset of the graph restricted to R  and the target
-        set A, we can show that it is a subset R. *)
-    with paritygame.tangle_attractor_ss[OF step(3) tangles_T\<^sub>\<alpha> fin_T\<^sub>\<alpha> step(8)] step(2)
-    show ?thesis by blast
-  qed
-  (** Since R' is obtained by removing Z from R, and we know that Z is a non-empty a subset of R,
-      R decreases monotonically with every step. *)
-  ultimately show ?case using step(13) by auto
-qed
-
-(** Because R is finite and decreases with every step, search_step is a well-founded relation. *)
-lemma search_step_wellfounded: "wfP (search_step\<inverse>\<inverse>)"
-  unfolding wfP_def
-  apply (rule wf_subset[of "inv_image (finite_psubset) (\<lambda>(R,Y). R)"]; clarsimp)
-  subgoal for R' Y' R Y
-    using search_step_R_anti_mono[of "(R,Y)" "(R',Y')"] search_step_R_finite[of "(R,Y)"]
-    by simp
-  done
-
-(** If R is a valid non-empty subgame, then search_step can always be applied.
-    The specifics of Y are not relevant, as it has no preconditions in the step. *)
-lemma search_step_continues_on_valid_R:
-  "\<lbrakk>R \<noteq> {}; R \<subseteq> V; paritygame (Restr E R) (V\<inter>R) (V\<^sub>0\<inter>R)\<rbrakk> \<Longrightarrow> Domainp search_step (R,Y)"
-proof -
-  assume R_notempty: "R\<noteq>{}" and
-         R_in_V: "R \<subseteq> V" and
-         R_valid_subgame: "paritygame (Restr E R) (V\<inter>R) (V\<^sub>0\<inter>R)"
-  (** All we have to do is define the local variables with their conditions in the step. *)
-  moreover define p where "p = pr_set R"
-  moreover define \<alpha> where "\<alpha> = player_wins_pr p"
-  moreover define A where "A = {v. v\<in>R \<and> pr v = p}"
-  moreover define T\<^sub>\<alpha> where "T\<^sub>\<alpha> = {t. t \<in> T \<and> paritygame.tangle (Restr E R) (V\<inter>R) (V\<^sub>0\<inter>R) pr \<alpha> t}"
-  moreover from T\<^sub>\<alpha>_def have
-    tangles_T\<^sub>\<alpha>: "\<forall>t\<in>T\<^sub>\<alpha>. paritygame.tangle (Restr E R) (V\<inter>R) (V\<^sub>0\<inter>R) pr \<alpha> t" and
-    fin_T\<^sub>\<alpha>: "finite T\<^sub>\<alpha>"
-    using finite_subset[OF _ fin_T] by auto
-  moreover obtain Z \<sigma> where
-    "paritygame.tangle_attractor (Restr E R) (V\<inter>R) (V\<^sub>0\<inter>R) pr \<alpha> T\<^sub>\<alpha> A Z \<sigma>"
-    using paritygame.tangle_attractor_exists[OF R_valid_subgame tangles_T\<^sub>\<alpha> fin_T\<^sub>\<alpha>] by blast
-  moreover define V\<^sub>\<alpha> where "V\<^sub>\<alpha> = V_player \<alpha>"
-  moreover define V\<^sub>\<beta> where "V\<^sub>\<beta> = V_opponent \<alpha>"
-  moreover define Ov where
-    "Ov = {v. v \<in> V\<^sub>\<alpha>\<inter>A \<and> E `` {v} \<inter> Z \<noteq> {}} \<union> {v. v \<in> V\<^sub>\<beta>\<inter>A \<and> (E `` {v}) \<inter> R \<subseteq> Z}"
-  moreover define Y' where "Y' = (if Ov \<noteq> {} then
-      Y \<union> {S. S \<subseteq> Z \<and> finite_graph_V_Succ.nt_bottom_SCC (induced_subgraph V\<^sub>\<alpha> \<sigma>) (induced_subgraph_V V\<^sub>\<alpha> \<sigma>) S}
-   else
-      Y)"
-  moreover define R' where "R' = R-Z"
-  (** Now, we can put them in their place in the step, and our thesis follows automatically. *)
-  ultimately have "search_step (R,Y) (R',Y')"
-    using search_step.step by blast
-  thus ?thesis by blast
-qed
-
-(** If we start from a valid, non-empty subgame, through applying search_step, we will always reach
-    a final state with a corresponding Y. *)
-lemma search_step_terminates_with_Y:
-  "\<lbrakk>fst S \<noteq> {}; fst S \<subseteq> V; paritygame (Restr E (fst S)) (V\<inter>fst S) (V\<^sub>0\<inter>fst S)\<rbrakk>
-  \<Longrightarrow> \<exists>Y. search_step\<^sup>*\<^sup>* S ({},Y)"
-  using search_step_wellfounded
-  unfolding wfP_def
-proof (induction S rule: wf_induct_rule)
-  case (less x)
-  (** Because R in x is a valid non-empty subgame, we know there is a state y that succeeds
-      it in search_step. *)
-  from search_step_continues_on_valid_R[OF less.prems, of "snd x"]
-  have "Domainp search_step x" by simp
-  then obtain y where step_x_y: "search_step x y" by blast
-  (** Now we consider whether R' in the successor y is empty or not. *)
-  consider (empty_R') "fst y = {}" | (nonempty_R') "fst y \<noteq> {}" by blast
-  thus ?case proof cases
-    (** If R' in y is already empty, we clearly have a step from x to an endpoint. *)
-    case empty_R'
-    with step_x_y have "search_step x ({}, snd y)"
-      using surjective_pairing[of y] by auto
-    thus ?thesis by blast
-  next
-    (** If R' is not empty, then we know it is a valid subgame in V by the properties of the
-        step. *)
-    case nonempty_R'
-    moreover from search_step_R_in_V[OF step_x_y] have "fst y \<subseteq> V" ..
-    moreover from step_result_R_is_paritygame[OF step_x_y]
-    have "paritygame (Restr E (fst y)) (V \<inter> fst y) (V\<^sub>0 \<inter> fst y)" .
-    moreover note step_x_y
-    (** By the induction hypothesis, we then know that from y, we can reach a state with an empty
-        R and a valid Y.*)
-    ultimately obtain Y where "search_step\<^sup>*\<^sup>* y ({}, Y)"
-      using less.IH by blast
-    (** We also know you can reach y from x. By the transitivity of the reflexive transitive
-        closure, we can now say that we can reach the state with an empty R from x, via y. *)
-    moreover from step_x_y have "search_step\<^sup>*\<^sup>* x y" by simp
-    ultimately show ?thesis using rtranclp_trans by fast
-  qed
-qed
-
-(** When an empty R is reached, there exist no further steps in the algorithm. *)
-lemma search_terminates_on_empty_R: "\<not>Domainp search_step ({},Y)"
-  using search_step_R_anti_mono[of "({},Y)"]
-  by auto
-*)
-
-(** TODO: invariant, prove property of Y on termination. *)
-(** The current invariant states that everything contained in Y is a tangle.
-    This should probably be restated to say that everything contained in Y is a tangle with its
-    corresponding strategy. *)
-(**
-definition search_I ::  "'v set \<times> 'v set set \<Rightarrow> bool" where
-  "search_I S \<equiv> finite (snd S) \<and> (\<forall>U \<in> snd S. \<exists>\<alpha>. tangle \<alpha> U) \<and> (fst S={} \<longrightarrow> \<dots>)"
-*)
-
-definition search_I :: "'v set \<times> 'v set set \<Rightarrow> bool" where
-  "search_I \<equiv> \<lambda>(R,Y). finite R \<and> valid_subgame R \<and> finite Y \<and> (\<forall>U \<in> Y. \<exists>\<alpha>. tangle \<alpha> U \<and> U \<notin> T)"
-
-(** If we end with an empty region, then we have a finite, non-empty Y containing new tangles that
-    were not included in T before, as specified by our invariant. *)
-lemma search_I_correct:
-  "search_I ({},Y) \<Longrightarrow> finite Y \<and> Y \<noteq> {} \<and> (\<forall>U \<in> Y. \<exists>\<alpha>. tangle \<alpha> U \<and> U \<notin> T)"
-  unfolding search_I_def apply simp sorry
 
 (** If our invariant holds for a state, a step of the search algorithm gives us a finite Y'. *)
 lemma search_step_finite_Y:
@@ -376,9 +257,10 @@ qed
 lemma search_step_I:
   "\<lbrakk>search_step (R,Y) (R',Y'); search_I (R,Y)\<rbrakk> \<Longrightarrow> search_I (R',Y')"
   using search_step_R_finite[of R Y R' Y']
-    search_step_valid_subgame search_step_finite_Y[of R Y R' Y']
+    search_step_valid_subgame
+    search_step_finite_Y[of R Y R' Y']
     search_step_tangles_Y[of R Y R' Y']
-  unfolding search_I_def by blast
+  unfolding search_I_def split by blast
 
 (** If two states are in the reflexive transitive closure of steps, then our invariant is preserved
     between them. *)
@@ -388,12 +270,6 @@ lemma search_step_rtranclp_I:
   subgoal by simp
   subgoal for y z using search_step_I[of "fst y" "snd y" "fst z" "snd z"] by simp
   done
-
-(** The search algorithm applies the search_step until it reaches the end.
-    We do not have to specify that ({},Y) is not in the domain of the step,
-    as this follows automatically because no further steps exist from an empty R. *)
-definition search :: "'v set \<Rightarrow> 'v set set \<Rightarrow> bool" where
-  "search R Y \<equiv> search_step\<^sup>*\<^sup>* (R,{}) ({},Y)"
 
 (**
 (** For every valid, non-empty subgame R, the search algorithm finds a Y. *)
@@ -422,6 +298,139 @@ lemma search_preserves_I:
 lemma valid_subgame_search_correct:
   "\<lbrakk>valid_subgame R; search R Y\<rbrakk> \<Longrightarrow> finite Y \<and> Y \<noteq> {} \<and> (\<forall>U \<in> Y. \<exists>\<alpha>. tangle \<alpha> U \<and> U \<notin> T)"
   using search_I_correct[OF search_preserves_I[OF _ I_base_valid_subgame]] by simp
+
+
+section \<open>Termination\<close>
+
+lemma search_step_wfP: "wfP (search_step\<inverse>\<inverse>)"
+  sorry
+
+(*
+(** search_step is inversely monotonous on R: R strictly decreases with every step. *)
+lemma search_step_R_anti_mono: "search_step S S' \<Longrightarrow> fst S' \<subset> fst S"
+proof (induction rule: search_step.induct)
+  case (step R p \<alpha> A T\<^sub>\<alpha> Z \<sigma> V\<^sub>\<alpha> V\<^sub>\<beta> Ov Y' Y R')
+  (** We know that every t in T\<^sub>\<alpha> is a tangle in the subgame of R, and that T\<^sub>\<alpha> is finite. We need
+      these properties for showing the next two properties. *)
+  from step(7) have tangles_T\<^sub>\<alpha>: "\<forall>t\<in>T\<^sub>\<alpha>. paritygame.tangle (Restr E R) (V \<inter> R) (V\<^sub>0 \<inter> R) pr \<alpha> t"
+    by blast
+  from step(7) have fin_T\<^sub>\<alpha>: "finite T\<^sub>\<alpha>"
+    using finite_subset[OF _ fin_T] by simp
+  (** We show that Z is not empty. *)
+  have "Z \<noteq> {}" proof -
+    (** R is finite *)
+    from finite_subset[OF step(2) fin_V] have fin_R: "finite R" .
+    (** A is part of the finite non-empty set R, therefore, it must contain at least one node
+        with priority p, and thus it is not empty. *)
+    from step(6) step(4) have "A \<noteq> {}"
+      using pr_set_exists[OF fin_R step(1)] by blast
+    (** Since the target A is part of the tangle-attracted region Z, Z must also be non-empty. *)
+    with paritygame.target_in_tangle_attractor[OF step(3) tangles_T\<^sub>\<alpha> fin_T\<^sub>\<alpha> step(8)]
+    show ?thesis by auto
+  qed
+  (** Furthermore, Z is a subset of of R. *)
+  moreover have "Z \<subseteq> R" proof -
+    from step(6) have A_in_R: "A \<subseteq> R" by simp
+    (** Since the tangle-attracted Z region is a subset of the graph restricted to R  and the target
+        set A, we can show that it is a subset R. *)
+    with paritygame.tangle_attractor_ss[OF step(3) tangles_T\<^sub>\<alpha> fin_T\<^sub>\<alpha> step(8)] step(2)
+    show ?thesis by blast
+  qed
+  (** Since R' is obtained by removing Z from R, and we know that Z is a non-empty a subset of R,
+      R decreases monotonically with every step. *)
+  ultimately show ?case using step(13) by auto
+qed
+
+(** Because R is finite and decreases with every step, search_step is a well-founded relation. *)
+lemma search_step_wellfounded: "wfP (search_step\<inverse>\<inverse>)"
+  unfolding wfP_def
+  apply (rule wf_subset[of "inv_image (finite_psubset) (\<lambda>(R,Y). R)"]; clarsimp)
+  subgoal for R' Y' R Y
+    using search_step_R_anti_mono[of "(R,Y)" "(R',Y')"] search_step_R_finite[of "(R,Y)"]
+    by simp
+  done
+
+(** If R is a valid non-empty subgame, then search_step can always be applied.
+    The specifics of Y are not relevant, as it has no preconditions in the step. *)
+lemma search_step_continues_on_valid_R:
+  "\<lbrakk>R \<noteq> {}; R \<subseteq> V; paritygame (Restr E R) (V\<inter>R) (V\<^sub>0\<inter>R)\<rbrakk> \<Longrightarrow> Domainp search_step (R,Y)"
+proof -
+  assume R_notempty: "R\<noteq>{}" and
+         R_in_V: "R \<subseteq> V" and
+         R_valid_subgame: "paritygame (Restr E R) (V\<inter>R) (V\<^sub>0\<inter>R)"
+  (** All we have to do is define the local variables with their conditions in the step. *)
+  moreover define p where "p = pr_set R"
+  moreover define \<alpha> where "\<alpha> = player_wins_pr p"
+  moreover define A where "A = {v. v\<in>R \<and> pr v = p}"
+  moreover define T\<^sub>\<alpha> where "T\<^sub>\<alpha> = {t. t \<in> T \<and> paritygame.tangle (Restr E R) (V\<inter>R) (V\<^sub>0\<inter>R) pr \<alpha> t}"
+  moreover from T\<^sub>\<alpha>_def have
+    tangles_T\<^sub>\<alpha>: "\<forall>t\<in>T\<^sub>\<alpha>. paritygame.tangle (Restr E R) (V\<inter>R) (V\<^sub>0\<inter>R) pr \<alpha> t" and
+    fin_T\<^sub>\<alpha>: "finite T\<^sub>\<alpha>"
+    using finite_subset[OF _ fin_T] by auto
+  moreover obtain Z \<sigma> where
+    "paritygame.tangle_attractor (Restr E R) (V\<inter>R) (V\<^sub>0\<inter>R) pr \<alpha> T\<^sub>\<alpha> A Z \<sigma>"
+    using paritygame.tangle_attractor_exists[OF R_valid_subgame tangles_T\<^sub>\<alpha> fin_T\<^sub>\<alpha>] by blast
+  moreover define V\<^sub>\<alpha> where "V\<^sub>\<alpha> = V_player \<alpha>"
+  moreover define V\<^sub>\<beta> where "V\<^sub>\<beta> = V_opponent \<alpha>"
+  moreover define Ov where
+    "Ov = {v. v \<in> V\<^sub>\<alpha>\<inter>A \<and> E `` {v} \<inter> Z \<noteq> {}} \<union> {v. v \<in> V\<^sub>\<beta>\<inter>A \<and> (E `` {v}) \<inter> R \<subseteq> Z}"
+  moreover define Y' where "Y' = (if Ov \<noteq> {} then
+      Y \<union> {S. S \<subseteq> Z \<and> finite_graph_V_Succ.nt_bottom_SCC (induced_subgraph V\<^sub>\<alpha> \<sigma>) (induced_subgraph_V V\<^sub>\<alpha> \<sigma>) S}
+   else
+      Y)"
+  moreover define R' where "R' = R-Z"
+  (** Now, we can put them in their place in the step, and our thesis follows automatically. *)
+  ultimately have "search_step (R,Y) (R',Y')"
+    using search_step.step by blast
+  thus ?thesis by blast
+qed
+
+(** If we start from a valid, non-empty subgame, through applying search_step, we will always reach
+    a final state with a corresponding Y. *)
+lemma search_step_terminates_with_Y:
+  "\<lbrakk>fst S \<noteq> {}; fst S \<subseteq> V; paritygame (Restr E (fst S)) (V\<inter>fst S) (V\<^sub>0\<inter>fst S)\<rbrakk>
+  \<Longrightarrow> \<exists>Y. search_step\<^sup>*\<^sup>* S ({},Y)"
+  using search_step_wellfounded
+  unfolding wfP_def
+proof (induction S rule: wf_induct_rule)
+  case (less x)
+  (** Because R in x is a valid non-empty subgame, we know there is a state y that succeeds
+      it in search_step. *)
+  from search_step_continues_on_valid_R[OF less.prems, of "snd x"]
+  have "Domainp search_step x" by simp
+  then obtain y where step_x_y: "search_step x y" by blast
+  (** Now we consider whether R' in the successor y is empty or not. *)
+  consider (empty_R') "fst y = {}" | (nonempty_R') "fst y \<noteq> {}" by blast
+  thus ?case proof cases
+    (** If R' in y is already empty, we clearly have a step from x to an endpoint. *)
+    case empty_R'
+    with step_x_y have "search_step x ({}, snd y)"
+      using surjective_pairing[of y] by auto
+    thus ?thesis by blast
+  next
+    (** If R' is not empty, then we know it is a valid subgame in V by the properties of the
+        step. *)
+    case nonempty_R'
+    moreover from search_step_R_in_V[OF step_x_y] have "fst y \<subseteq> V" ..
+    moreover from step_result_R_is_paritygame[OF step_x_y]
+    have "paritygame (Restr E (fst y)) (V \<inter> fst y) (V\<^sub>0 \<inter> fst y)" .
+    moreover note step_x_y
+    (** By the induction hypothesis, we then know that from y, we can reach a state with an empty
+        R and a valid Y.*)
+    ultimately obtain Y where "search_step\<^sup>*\<^sup>* y ({}, Y)"
+      using less.IH by blast
+    (** We also know you can reach y from x. By the transitivity of the reflexive transitive
+        closure, we can now say that we can reach the state with an empty R from x, via y. *)
+    moreover from step_x_y have "search_step\<^sup>*\<^sup>* x y" by simp
+    ultimately show ?thesis using rtranclp_trans by fast
+  qed
+qed
+
+(** When an empty R is reached, there exist no further steps in the algorithm. *)
+lemma search_terminates_on_empty_R: "\<not>Domainp search_step ({},Y)"
+  using search_step_R_anti_mono[of "({},Y)"]
+  by auto
+*)
 end (** End of context with fixed T. *)
 
 end (** End of context paritygame *)
